PktClass.v
@@ -176,7 +176,7 @@ Definition linear_db (db : FilterDatabase) : GeneralCaracaraProgram :=
   let t := List.fold_right
     (fun '(f, lbl) acc =>
       let mp := FlattenFilter f in
-      let new_rule := Seq (SeqCtr mp [StatelessOp AddOp (ConstantArg (CrUInt8 lbl)) (ConstantArg (CrUInt8 (repr 0))) h_out]) in
+      let new_rule := Seq (SeqCtr mp [StatelessOp AddOp u8 (OpConst (CrInt (repr (unsigned lbl)))) (OpConst (CrInt (repr 0))) h_out]) in
       new_rule :: acc)
     [] db' in
   let p := CaracaraProgramDef [h_out] [] [] t in
@@ -190,7 +190,7 @@ Definition linear_db (db : FilterDatabase) : GeneralCaracaraProgram :=
 Definition interp (ps : ConcreteState) : option Label :=
   match (header_map ps) !! 1 with
   | IntVal n => match n with
-    | CrUInt8 lbl => Some lbl
+    | CrInt lbl => Some (repr (unsigned lbl))
     | _ => None
     end
   | _ => None
@@ -236,14 +236,14 @@ Definition make_table_transformer (table : FilterDatabase) (h_body : Header): Tr
   List.map (fun '(f, lbl) =>
     Seq (SeqCtr (FlattenFilter f)
       [StatelessOp
-        AddOp
-        (ConstantArg (CrUInt8 lbl))
-        (ConstantArg (CrUInt8 (repr 0)))
+        AddOp u8
+        (OpConst (CrInt (repr (unsigned lbl))))
+        (OpConst (CrInt (repr 0)))
         (h_body);
       StatelessOp
-        AddOp
-        (ConstantArg (CrUInt8 (repr (Zpos (priority f)))))
-        (ConstantArg (CrUInt8 (repr 0)))
+        AddOp u8
+        (OpConst (CrInt (repr (Zpos (priority f)))))
+        (OpConst (CrInt (repr 0)))
         (incr h_body)])
   ) sorted.
 
@@ -254,14 +254,14 @@ Definition check_match (acc_base : Header) (filter_base : Header) : Transformer 
   [Seq (SeqCtr
     [((incr acc_base), CmpLt, MatchHeader (incr filter_base))]
     [StatelessOp
-      AddOp
-      (HeaderArg filter_base)
-      (ConstantArg (CrUInt8 (repr 0)))
+      AddOp u8
+      (OpHeader filter_base)
+      (OpConst (CrInt (repr 0)))
       acc_base;
     StatelessOp
-      AddOp
-      (HeaderArg (incr filter_base))
-      (ConstantArg (CrUInt8 (repr 0)))
+      AddOp u8
+      (OpHeader (incr filter_base))
+      (OpConst (CrInt (repr 0)))
       (incr acc_base)
     ])].
 
@@ -341,20 +341,20 @@ Definition tss_db (db : FilterDatabase) : GeneralCaracaraProgram :=
 
 Definition SimpleDB : FilterDatabase :=
   [({|
-      src_ip := [(HeaderCtr 1, CmpEq, MatchConst (CrUInt8 (repr 0)))];
-      dst_ip := [(HeaderCtr 5, CmpEq, MatchConst (CrUInt8 (repr 0)))];
-      src_port := [(HeaderCtr 9, CmpEq, MatchConst (CrUInt8 (repr 0)))];
-      dst_port := [(HeaderCtr 11, CmpEq, MatchConst (CrUInt8 (repr 0)))];
-      protocol := [(HeaderCtr 13, CmpEq, MatchConst (CrUInt8 (repr 1)))];
+      src_ip := [(HeaderCtr 1, CmpEq, MatchConst (CrInt (repr 0)))];
+      dst_ip := [(HeaderCtr 5, CmpEq, MatchConst (CrInt (repr 0)))];
+      src_port := [(HeaderCtr 9, CmpEq, MatchConst (CrInt (repr 0)))];
+      dst_port := [(HeaderCtr 11, CmpEq, MatchConst (CrInt (repr 0)))];
+      protocol := [(HeaderCtr 13, CmpEq, MatchConst (CrInt (repr 1)))];
       key := 1%positive;
       priority := 1%positive |}, (repr 42));
     ({|
-      src_ip := [(HeaderCtr 1, CmpEq, MatchConst (CrUInt8 (repr 0)));
-                 (HeaderCtr 2, CmpEq, MatchConst (CrUInt8 (repr 0)))];
-      dst_ip := [(HeaderCtr 5, CmpEq, MatchConst (CrUInt8 (repr 0)))];
-      src_port := [(HeaderCtr 9, CmpEq, MatchConst (CrUInt8 (repr 0)))];
-      dst_port := [(HeaderCtr 11, CmpEq, MatchConst (CrUInt8 (repr 0)))];
-      protocol := [(HeaderCtr 13, CmpEq, MatchConst (CrUInt8 (repr 2)))];
+      src_ip := [(HeaderCtr 1, CmpEq, MatchConst (CrInt (repr 0)));
+                 (HeaderCtr 2, CmpEq, MatchConst (CrInt (repr 0)))];
+      dst_ip := [(HeaderCtr 5, CmpEq, MatchConst (CrInt (repr 0)))];
+      src_port := [(HeaderCtr 9, CmpEq, MatchConst (CrInt (repr 0)))];
+      dst_port := [(HeaderCtr 11, CmpEq, MatchConst (CrInt (repr 0)))];
+      protocol := [(HeaderCtr 13, CmpEq, MatchConst (CrInt (repr 2)))];
       key := 2%positive;
       priority := 2%positive
     |}, (repr 67))
